sketch using wf-ness

dev2015/dot-smallstep3b.v
@@ -1,5 +1,5 @@
 (* smallstep proof *)
-(* compared to 3a, makes has_type independent of vtp *)
+(* compared to 3a2, makes tobj recursive (still only one member) *)
 
 Require Export SfLib.
 
@@ -112,11 +112,17 @@ Fixpoint subst (U : ty) (T : ty) {struct T} : ty :=
   end.
 
 
+Fixpoint dms_curry (d: dm) : ty :=
+  match d with
+    | dty T => TMem T T
+    | dfun T1 T2 _ => TFun T1 T2
+  end.
 
 Inductive has_type : tenv -> venv -> tm -> ty -> nat -> Prop :=
   | T_Varx : forall GH G1 x ds T n1,
       index x G1 = Some (vobj ds) ->
-      dms_has_type [] G1 ds T n1 ->
+      dms_curry ds = T -> (* poor man's store typing *)
+      closed 0 (length G1) 0 T ->
       has_type GH G1 (tvar true x) T (S n1)
   | T_Vary : forall G1 GH x T n1,
       index x GH = Some T ->
@@ -132,11 +138,11 @@ Inductive has_type : tenv -> venv -> tm -> ty -> nat -> Prop :=
       T1' = (open 0 (TVar b x) T1) ->
       closed (length GH) (length G1) 0 T1' ->
       has_type GH G1 (tvar b x) T1' (S n1)
-(* todo: make tobj recursive *)
-  | T_Obj : forall GH G1 ds T n1,
-      dms_has_type GH G1 ds T n1 ->
-      closed (length GH) (length G1) 0 T ->
-      has_type GH G1 (tobj ds) T (S n1)
+  | T_Obj : forall GH G1 ds T T' n1,
+      dms_has_type (T'::GH) G1 ds T' n1 ->
+      closed (length GH) (length G1) 1 T ->
+      T' = open 0 (TVar false (length GH)) T ->
+      has_type GH G1 (tobj ds) (TBind T) (S n1)
   | T_App : forall T1 T2 GH G1 t1 t2 n1 n2,
       has_type GH G1 t1 (TFun T1 T2) n1 ->
       has_type GH G1 t2 T1 n2 ->
@@ -522,11 +528,11 @@ Proof.
   - eapply htp_bind. eapply IHn. eauto. omega. eapply closed_extend. eauto. 
   - eapply htp_sub. eapply IHn. eauto. omega. eapply IHn. eauto. omega. eauto. eauto.
   (* has_type *)
-  - econstructor. eapply index_extend. eauto. eapply IHn. eauto. omega.
+  - econstructor. eapply index_extend. eauto. eauto. eapply closed_extend. eauto.
   - econstructor. eauto. eapply closed_extend. eauto.
   - econstructor. eapply IHn. eauto. omega. eauto. eapply closed_extend. eauto.
   - econstructor. eapply IHn. eauto. omega. eauto. eapply closed_extend. eauto.
-  - econstructor. eapply IHn. eauto. omega. eapply closed_extend. eauto.
+  - econstructor. eapply IHn. eauto. omega. eapply closed_extend. eauto. eauto.
   - econstructor. subst. eapply IHn. eauto. omega. eapply IHn. eauto. omega. eapply closed_extend. eauto.
   - eapply T_AppVar. eapply IHn. eauto. omega. eapply IHn. eauto. omega. eauto. eapply closed_extend. eauto.
   - econstructor. eapply IHn. eauto. omega. eapply IHn. eauto. omega.
@@ -655,11 +661,11 @@ Proof.
   - eapply IHH1 in H1. eapply closed_open. simpl. eapply closed_upgrade_gh. eauto. omega. econstructor. eauto. omega. 
   - eapply closed_upgrade_gh. eapply IHS2. eauto. omega. rewrite H4. rewrite app_length. omega. 
   (* has_type *)
-  - eapply closed_upgrade_gh. eapply IHD. eauto. omega. simpl. omega.
+  - subst. eapply closed_upgrade_gh. eauto. omega.
   - eauto.
   - econstructor. eapply closed_upgrade_gh. eauto. omega.
   - eapply IHT in H1. inversion H1; subst. eauto. omega.
-  - eapply IHD in H1. eauto. omega.
+  - econstructor. eauto.
   - eapply IHT in H1. inversion H1. eauto. omega.
   - eapply IHT in H1. inversion H1. eauto. omega.
   - eapply IHS2. eauto. omega.
@@ -1803,40 +1809,27 @@ Inductive step : venv -> tm -> venv -> tm -> Prop :=
     step G1 (tapp (tvar true f) t2) G1' (tapp (tvar true f) t2')
 .
 
-
+Definition wf_sto_at x (G1: venv) :=
+  forall ds, index x G1 = Some (vobj ds) -> exists m n, vtp m G1 x (dms_curry ds) n.
 
 Lemma hastp_inv: forall G1 x T n1,
+  wf_sto_at x G1 ->
   has_type [] G1 (tvar true x) T n1 ->
   exists m n1, vtp m G1 x T n1.
 Proof.
-  intros. remember [] as GH. remember (tvar true x) as t.
+  intros G1 x T n1 Hwf H. remember [] as GH. remember (tvar true x) as t.
   induction H; subst; try inversion Heqt.
-  - Case "varx". subst. inversion H0; subst.
-    + assert (stpd2 [] G1 T11 T11) as A. {
-        eapply stpd2_refl. eauto.
-      }
-      eu. repeat eexists. eapply vtp_mem. eauto. eauto. eauto.
-    + assert (stpd2 [] G1 T11 T11) as A. {
-        eapply stpd2_refl. eauto.
-      }
-      assert (stpd2 [T11] G1 (open 0 (TVar false 0) T12) (open 0 (TVar false 0) T12)) as B. {
-        eapply stpd2_refl. eapply closed_open. eapply closed_upgrade_gh. eauto.
-        simpl. omega. simpl. econstructor. omega.
-      }
-      eu. eu. repeat eexists. eapply vtp_fun.
-      eauto. eauto. eauto. eauto. eauto. eauto. eauto. eauto.
+  - Case "varx". subst. unfold wf_sto_at in Hwf. eapply Hwf. eauto.
   - Case "pack". subst.
-    destruct IHhas_type. eauto. eauto. ev.
+    destruct IHhas_type. eauto. eauto. eauto. ev.
     repeat eexists. eapply vtp_bind. eauto. eauto.
   - Case "unpack". subst.
-    destruct IHhas_type. eauto. eauto. ev. inversion H0.
+    destruct IHhas_type. eauto. eauto. auto. ev. inversion H0.
     repeat eexists. eauto.
   - Case "sub".
-    destruct IHhas_type. eauto. eauto. ev.
+    destruct IHhas_type. eauto. eauto. eauto. ev.
     assert (exists m0, vtpdd m0 G1 x T2). eexists. eapply vtp_widen; eauto. 
     ev. eu. repeat eexists. eauto. 
-Grab Existential Variables.
-apply 0. apply 0.
 Qed.
 
 Lemma stp2_subst_narrow: forall GH0 TX G1 T1 T2 x m n1 n2,
@@ -1863,26 +1856,26 @@ Qed.
 
 Lemma hastp_subst_aux: forall ni, (forall G1 GH TX T x t n1 n2,
   has_type (GH++[TX]) G1 t T n2 -> n2 < ni ->
-  has_type [] G1 (tvar true x) TX n1 ->
+  has_type [] G1 (tvar true x) TX n1 -> wf_sto_at x G1 ->
   exists n3, has_type (map (substt x) GH) G1 (subst_tm x t) (substt x T) n3) /\
   (forall G1 GH TX T x ds n1 n2,
   dms_has_type (GH++[TX]) G1 ds T n2 -> n2 < ni ->
-  has_type [] G1 (tvar true x) TX n1 ->
+  has_type [] G1 (tvar true x) TX n1 -> wf_sto_at x G1 ->
   exists n3, dms_has_type (map (substt x) GH) G1 (subst_dm x ds) (substt x T) n3).
 Proof.
   intro ni. induction ni. split; intros; omega. destruct IHni as [IHniT IHniD].
   split;
   intros; remember (GH++[TX]) as GH0; revert GH HeqGH0; inversion H; intros.
-  - Case "varx". subst. simpl. eexists. eapply T_Varx. eauto. erewrite subst_closed_id. eauto. eapply dms_has_type_closed in H3. eauto.
+  - Case "varx". subst. simpl. eexists. eapply T_Varx. eauto. erewrite subst_closed_id. eauto. eauto. eapply closed_subst. eapply closed_upgrade_gh. eauto. omega. econstructor. eapply has_type_closed1. eauto.
   - Case "vary". subst. simpl.
     case_eq (beq_nat x0 0); intros E.
     + assert (x0 = 0). eapply beq_nat_true_iff; eauto. subst x0.
-      eapply index_hit0 in H2. subst.  erewrite subst_closed_id.
+      eapply index_hit0 in H3. subst.  erewrite subst_closed_id.
       eapply hastp_upgrade_gh. eauto. eapply has_type_closed in H1. eauto.
     + assert (x0 <> 0). eapply beq_nat_false_iff; eauto.
-      eexists. eapply T_Vary. eapply index_subst1. eauto. eauto. rewrite map_length. eapply closed_subst0. rewrite app_length in H3. simpl in H3. eapply H3. eapply has_type_closed1. eauto.
+      eexists. eapply T_Vary. eapply index_subst1. eauto. eauto. rewrite map_length. eapply closed_subst0. rewrite app_length in H4. simpl in H4. eapply H4. eapply has_type_closed1. eauto.
   - Case "pack". subst. simpl.
-    edestruct IHniT as [? IH]. eauto. omega. eauto. 
+    edestruct IHniT as [? IH]. eauto. omega. eauto. eauto.
     assert (substt x (TBind T1) = (TBind (substt x T1))) as A. {
       eauto.
     }
@@ -1890,30 +1883,30 @@ Proof.
     destruct b.
     + eexists. eapply T_VarPack. eapply IH.
       unfold substt. rewrite subst_open_commute1. reflexivity.
-      rewrite map_length. eapply closed_subst0. rewrite app_length in H4. simpl in H4.
-      apply H4. eapply has_type_closed1. eauto.
+      rewrite map_length. eapply closed_subst0. rewrite app_length in H5. simpl in H5.
+      apply H5. eapply has_type_closed1. eauto.
     + case_eq (beq_nat x0 0); intros E.
       * assert (x0 = 0). eapply beq_nat_true_iff; eauto. subst x0.
         simpl in IH.
         eexists. eapply T_VarPack. eapply IH. rewrite subst_open_commute0b. eauto.
-        rewrite map_length. eapply closed_subst. rewrite app_length in H4. simpl in H4.
-        eapply H4. econstructor. eapply has_type_closed1. eauto.
+        rewrite map_length. eapply closed_subst. rewrite app_length in H5. simpl in H5.
+        eapply H5. econstructor. eapply has_type_closed1. eauto.
       * assert (x0 <> 0). eapply beq_nat_false_iff; eauto.
         simpl in IH. rewrite E in IH.
         eexists. eapply T_VarPack. eapply IH.
         remember (x0 - 1) as z.
         assert (x0 = z + 1) as B. {
-          intuition. destruct x0. specialize (H3 eq_refl). inversion H3.
+          intuition. destruct x0. specialize (H4 eq_refl). inversion H4.
           subst. simpl. rewrite <- minus_n_O. rewrite NPeano.Nat.add_1_r.
           reflexivity.
         }
         rewrite B. unfold substt.
         rewrite subst_open_commute_z. reflexivity.
-        rewrite map_length. eapply closed_subst. rewrite app_length in H4.
-        simpl in H4. eapply H4.
+        rewrite map_length. eapply closed_subst. rewrite app_length in H5.
+        simpl in H5. eapply H5.
         econstructor. eapply has_type_closed1. eauto.
   - Case "unpack". subst. simpl.
-    edestruct IHniT as [? IH]. eapply H2. omega. eauto.
+    edestruct IHniT as [? IH]. eapply H3. omega. eauto. eauto.
     assert (substt x (TBind T1) = (TBind (substt x T1))) as A. {
       eauto.
     }
@@ -1921,40 +1914,45 @@ Proof.
     destruct b.
     + eexists. eapply T_VarUnpack. eapply IH.
       unfold substt. rewrite subst_open_commute1. reflexivity.
-      rewrite map_length. eapply closed_subst0. rewrite app_length in H4. simpl in H4.
-      apply H4. eapply has_type_closed1. eauto.
+      rewrite map_length. eapply closed_subst0. rewrite app_length in H5. simpl in H5.
+      apply H5. eapply has_type_closed1. eauto.
     + case_eq (beq_nat x0 0); intros E.
       * assert (x0 = 0). eapply beq_nat_true_iff; eauto. subst x0.
         simpl in IH.
         eexists. eapply T_VarUnpack. eapply IH. rewrite subst_open_commute0b. eauto.
-        rewrite map_length. eapply closed_subst. rewrite app_length in H4. simpl in H4.
-        eapply H4. econstructor. eapply has_type_closed1. eauto.
+        rewrite map_length. eapply closed_subst. rewrite app_length in H5. simpl in H5.
+        eapply H5. econstructor. eapply has_type_closed1. eauto.
       * assert (x0 <> 0). eapply beq_nat_false_iff; eauto.
         simpl in IH. rewrite E in IH.
         eexists. eapply T_VarUnpack. eapply IH.
         remember (x0 - 1) as z.
         assert (x0 = z + 1) as B. {
-          intuition. destruct x0. specialize (H3 eq_refl). inversion H3.
+          intuition. destruct x0. specialize (H4 eq_refl). inversion H4.
           subst. simpl. rewrite <- minus_n_O. rewrite NPeano.Nat.add_1_r.
           reflexivity.
         }
         rewrite B. unfold substt.
         rewrite subst_open_commute_z. reflexivity.
-        rewrite map_length. eapply closed_subst. rewrite app_length in H4.
-        simpl in H4. eapply H4.
+        rewrite map_length. eapply closed_subst. rewrite app_length in H5.
+        simpl in H5. eapply H5.
         econstructor. eapply has_type_closed1. eauto.
-  - Case "obj". subst. simpl.
-    edestruct IHniD as [? IH]. eauto. omega. eauto.
-    eexists. eapply T_Obj. eauto. eapply dms_has_type_closed. eauto.
+  - Case "obj".
+    edestruct IHniD with (GH:=T'::GH1) as [? IH]. subst. eauto. omega. subst. eauto. subst. eauto.
+    subst. simpl.
+    eexists. eapply T_Obj. eauto.
+    eapply closed_subst. rewrite app_length in *. simpl in *. rewrite map_length. eauto.
+    econstructor. eapply has_type_closed1. eauto.
+    rewrite app_length. simpl. unfold substt. rewrite subst_open_commute_z.
+    rewrite map_length. eauto.
   - Case "app". subst. simpl.
-    edestruct IHniT as [? IH1]. eapply H2. omega. eauto.
-    edestruct IHniT as [? IH2]. eapply H3. omega. eauto.
+    edestruct IHniT as [? IH1]. eapply H3. omega. eauto. eauto.
+    edestruct IHniT as [? IH2]. eapply H4. omega. eauto. eauto.
     eexists. eapply T_App. eauto. eauto. eapply closed_subst.
     subst. rewrite map_length. rewrite app_length in *. simpl in *. eauto.
     subst. rewrite map_length. econstructor. eapply has_type_closed1. eauto.
   - Case "appvar". subst. simpl.
-    edestruct IHniT as [? IH1]. eapply H2. omega. eauto.
-    edestruct IHniT as [? IH2]. eapply H3. omega. eauto.
+    edestruct IHniT as [? IH1]. eapply H3. omega. eauto. eauto.
+    edestruct IHniT as [? IH2]. eapply H4. omega. eauto. eauto.
     destruct b2.
 
     eexists. eapply T_AppVar. eauto. eauto.
@@ -1982,37 +1980,70 @@ Proof.
     apply []. apply beq_nat_false. apply E. apply []. apply beq_nat_false. apply E.
   - Case "sub". subst.
     edestruct hastp_inv as [? [? HV]]; eauto.
-    edestruct stp2_subst_narrow. eapply H3. eapply HV.
-    edestruct IHniT as [? IH]. eapply H2. omega. eauto.
+    edestruct stp2_subst_narrow. eapply H4. eapply HV.
+    edestruct IHniT as [? IH]. eapply H3. omega. eauto. eauto.
     eexists. eapply T_Sub. eauto. eauto.
   - Case "mem". subst. simpl.
-    eexists. eapply D_Mem. eapply closed_subst0. rewrite app_length in H2. rewrite map_length. eauto. eapply has_type_closed1. eauto.
+    eexists. eapply D_Mem. eapply closed_subst0. rewrite app_length in H3. rewrite map_length. eauto. eapply has_type_closed1. eauto.
   - Case "abs". subst. simpl.
-    edestruct IHniT with (GH:=T11::GH1) as [? HI] . eauto. omega. eauto.
+    edestruct IHniT with (GH:=T11::GH1) as [? HI] . eauto. omega. eauto. eauto.
     simpl in HI. 
     eexists. eapply D_Abs. eapply HI.
     rewrite map_length. rewrite app_length. simpl.
     rewrite subst_open. unfold substt. reflexivity.
-    eapply closed_subst0. rewrite map_length. rewrite app_length in H4. simpl in H4. eauto. eauto. eapply has_type_closed1. eauto.
-    eapply closed_subst0. rewrite map_length. rewrite app_length in H5. simpl in H5. eauto. eapply has_type_closed1. eauto.
+    eapply closed_subst0. rewrite map_length. rewrite app_length in H5. simpl in H5. eauto. eauto. eapply has_type_closed1. eauto.
+    eapply closed_subst0. rewrite map_length. rewrite app_length in H6. simpl in H6. eauto. eapply has_type_closed1. eauto.
 Grab Existential Variables.
-apply 0. apply 0.
+apply 0. apply 0. apply 0.
 Qed.
 
 Lemma hastp_subst: forall G1 GH TX T x t n1 n2,
   has_type (GH++[TX]) G1 t T n2 ->
-  has_type [] G1 (tvar true x) TX n1 ->
+  has_type [] G1 (tvar true x) TX n1 -> wf_sto_at x G1 ->
   exists n3, has_type (map (substt x) GH) G1 (subst_tm x t) (substt x T) n3.
 Proof.
-  intros. eapply hastp_subst_aux with (t:=t). eauto. eauto. eauto.
+  intros. eapply hastp_subst_aux with (t:=t). eauto. eauto. eauto. eauto.
+Qed.
+
+Inductive wf_sto: venv -> Prop :=
+| wfs_nil : wf_sto nil
+| wfs_ext : forall G1 ds, wf_sto G1 ->
+                          (exists m n, vtp m ((vobj ds)::G1) (length G1) (dms_curry ds) n) ->
+                          wf_sto ((vobj ds)::G1).
+
+Lemma wf_sto_at_extends: forall G1 x vx v,
+  index x G1 = Some vx ->  
+  wf_sto_at x G1 -> wf_sto_at x (v::G1).
+Proof.
+  intros G1 x vx v. destruct vx as [dsx].
+  unfold wf_sto_at in *. intros HI Hwf.
+  specialize (Hwf dsx HI). intros.
+  eapply index_extend in HI. rewrite HI in H. inversion H. subst.
+  destruct Hwf as [m [n Hwf]]. exists m. exists n. eapply vtp_extend. eauto.
+Qed.
+
+Lemma wf_sto_at_bound: forall G1 x,
+  wf_sto G1 ->
+  x < length G1 ->
+  wf_sto_at x G1.
+Proof.
+  intros G1 x Hwf Le.
+  edestruct index_exists as [v HI]. eauto. clear Le. induction G1.
+  - inversion HI.
+  - simpl in HI. case_eq (beq_nat x (length G1)); intros E.
+    + rewrite E in HI. inversion HI. subst. inversion Hwf. subst.
+      unfold wf_sto_at. simpl. rewrite E. intros ? Hv. inversion Hv. subst.
+      eapply beq_nat_true in E. rewrite E. eauto.
+    + rewrite E in HI. eapply wf_sto_at_extends. eauto. eapply IHG1.
+      inversion Hwf; subst. eauto. eauto.
 Qed.
 
 Theorem type_safety : forall G t T n1,
-  has_type [] G t T n1 ->
+  has_type [] G t T n1 -> wf_sto G ->
   (exists x, t = tvar true x) \/
-  (exists G' t' n2, step G t (G'++G) t' /\ has_type [] (G'++G) t' T n2).
+  (exists G' t' n2, step G t (G'++G) t' /\ has_type [] (G'++G) t' T n2 /\ wf_sto (G'++G)).
 Proof. 
-  intros.
+  intros G t T n1 H Hwf.
   assert (closed (length ([]:tenv)) (length G) 0 T) as CL. eapply has_type_closed. eauto. 
   remember [] as GH. remember t as tt. remember T as TT.
   revert T t HeqTT HeqGH Heqtt CL. 
@@ -2025,32 +2056,32 @@ Proof.
   - Case "unpack". subst GH.
     eapply has_type_closed_b in H. destruct H. subst.
     left. eexists. reflexivity.
-  - Case "obj". subst. right.
+  - Case "obj". admit. (*subst. right.
     repeat eexists. rewrite <- app_cons1. eapply ST_Obj. eapply T_Varx.
     simpl. rewrite beq_nat_true_eq. eauto.
-    eapply dms_has_type_extend. eauto.
+    eapply dms_has_type_extend. eauto.*)
   - Case "app". subst.
     assert (closed (length ([]:tenv)) (length G1) 0 (TFun T1 T)) as TF. eapply has_type_closed. eauto. 
     assert ((exists x : id, t2 = tvar true x) \/
                 (exists (G' : venv) (t' : tm) n2,
-                   step G1 t2 (G'++G1) t' /\ has_type [] (G'++G1) t' T1 n2)) as HX.
-    eapply IHhas_type2. eauto. eauto. eauto. inversion TF. eauto. 
+                   step G1 t2 (G'++G1) t' /\ has_type [] (G'++G1) t' T1 n2 /\ wf_sto (G'++G1))) as HX.
+    eapply IHhas_type2. eauto. eauto. eauto. eauto. inversion TF. eauto. 
     assert ((exists x : id, t1 = tvar true x) \/
                 (exists (G' : venv) (t' : tm) n2,
-                   step G1 t1 (G'++G1) t' /\ has_type [] (G'++G1) t' (TFun T1 T) n2)) as HF.
-    eapply IHhas_type1. eauto. eauto. eauto. eauto.
+                   step G1 t1 (G'++G1) t' /\ has_type [] (G'++G1) t' (TFun T1 T) n2 /\ wf_sto (G'++G1))) as HF.
+    eapply IHhas_type1. eauto. eauto. eauto. eauto. eauto.
     destruct HF.
     + SCase "fun-val".
       destruct HX.
       * SSCase "arg-val".
         ev. ev. subst. 
-        assert (exists m n1, vtp m G1 x (TFun T1 T) n1). eapply hastp_inv. eauto.
-        assert (exists m n1, vtp m G1 x0 T1 n1). eapply hastp_inv. eauto.
+        assert (exists m n1, vtp m G1 x (TFun T1 T) n1). eapply hastp_inv. eapply wf_sto_at_bound. eauto. eapply has_type_closed1. eauto. eauto.
+        assert (exists m n1, vtp m G1 x0 T1 n1). eapply hastp_inv. eapply wf_sto_at_bound. eauto. eapply has_type_closed1. eauto. eauto.
         ev. inversion H2. subst.
         assert (vtpdd x1 G1 x0 T0). eapply vtp_widen. eauto. eauto. eauto. eauto. eauto.
         eu.
         assert (has_typed (map (substt x0) []) G1 (subst_tm x0 t) (substt x0 (open 0 (TVar false 0) T2))) as HI.
-        eapply hastp_subst; eauto.
+        eapply hastp_subst; eauto. eapply wf_sto_at_bound. eauto. eapply vtp_closed1. eauto.
         eu. simpl in HI.
         edestruct stp2_subst_narrow as [? HI2]. rewrite app_nil_l. eapply H17. eauto.
         simpl in HI2.
@@ -2060,23 +2091,23 @@ Proof.
         }
         rewrite EqT in HI2.
         right. repeat eexists. rewrite app_nil_l. eapply ST_AppAbs. eauto.
-        eapply T_Sub. eauto. eauto.
+        eapply T_Sub. eauto. eauto. eauto.
       * SSCase "arg_step".
         ev. subst. 
         right. repeat eexists. eapply ST_App2. eauto. eapply T_App.
         eapply has_type_extend_mult. eauto. eauto.
-        simpl in *. rewrite app_length. eapply closed_extend_mult. eassumption. omega.
+        simpl in *. rewrite app_length. eapply closed_extend_mult. eassumption. omega. eauto.
     + SCase "fun_step".
       ev. subst. right. repeat eexists. eapply ST_App1. eauto. eapply T_App.
       eauto. eapply has_type_extend_mult. eauto.
-      simpl in *. rewrite app_length. eapply closed_extend_mult. eassumption. omega.
+      simpl in *. rewrite app_length. eapply closed_extend_mult. eassumption. omega. eauto.
 
   - Case "appvar". subst.
     assert (closed (length ([]:tenv)) (length G1) 0 (TFun T1 T2)) as TF. eapply has_type_closed. eauto.
     assert ((exists x : id, tvar b2 x2 = tvar true x) \/
                 (exists (G' : venv) (t' : tm) n2,
-                   step G1 (tvar b2 x2) (G'++G1) t' /\ has_type [] (G'++G1) t' T1 n2)) as HX.
-    eapply IHhas_type2. eauto. eauto. eauto. inversion TF. eauto.
+                   step G1 (tvar b2 x2) (G'++G1) t' /\ has_type [] (G'++G1) t' T1 n2 /\ wf_sto (G'++G1))) as HX.
+    eapply IHhas_type2. eauto. eauto. eauto. eauto. inversion TF. eauto.
     assert (b2 = true) as HXeq. {
       destruct HX as [[? HX] | Contra]. inversion HX. reflexivity.
       destruct Contra as [G' [t' [n' [Hstep Htyp]]]].
@@ -2085,18 +2116,18 @@ Proof.
     clear HX. subst b2.
     assert ((exists x : id, t1 = tvar true x) \/
                 (exists (G' : venv) (t' : tm) n2,
-                   step G1 t1 (G'++G1) t' /\ has_type [] (G'++G1) t' (TFun T1 T2) n2)) as HF.
-    eapply IHhas_type1. eauto. eauto. eauto. eauto.
+                   step G1 t1 (G'++G1) t' /\ has_type [] (G'++G1) t' (TFun T1 T2) n2 /\ wf_sto (G'++G1))) as HF.
+    eapply IHhas_type1. eauto. eauto. eauto. eauto. eauto.
     destruct HF.
     + SCase "fun-val".
       ev. ev. subst.
-      assert (exists m n1, vtp m G1 x (TFun T1 T2) n1). eapply hastp_inv. eauto.
-      assert (exists m n1, vtp m G1 x2 T1 n1). eapply hastp_inv. eauto.
+      assert (exists m n1, vtp m G1 x (TFun T1 T2) n1). eapply hastp_inv. eapply wf_sto_at_bound. eauto. eapply has_type_closed1. eauto. eauto.
+      assert (exists m n1, vtp m G1 x2 T1 n1). eapply hastp_inv. eapply wf_sto_at_bound. eauto. eapply has_type_closed1. eauto. eauto.
       ev. inversion H1. subst.
       assert (vtpdd x0 G1 x2 T0). eapply vtp_widen. eauto. eauto. eauto. eauto. eauto.
       eu.
       assert (has_typed (map (substt x2) []) G1 (subst_tm x2 t) (substt x2 (open 0 (TVar false 0) T3))) as HI.
-      eapply hastp_subst; eauto.
+      eapply hastp_subst; eauto. eapply wf_sto_at_bound. eauto. eapply vtp_closed1. eauto.
       eu. simpl in HI.
       edestruct stp2_subst_narrow as [? HI2]. rewrite app_nil_l. eapply H17. eauto.
       simpl in HI2.
@@ -2106,23 +2137,23 @@ Proof.
       }
       rewrite EqT2 in HI2.
       right. repeat eexists. rewrite app_nil_l. eapply ST_AppAbs. eauto.
-      eapply T_Sub. eauto. eauto.
+      eapply T_Sub. eauto. eauto. eauto.
     + SCase "fun_step".
       ev. subst. right. repeat eexists. eapply ST_App1. eauto. eapply T_AppVar.
       eauto. eapply has_type_extend_mult. eauto. reflexivity.
-      simpl in *. rewrite app_length. eapply closed_extend_mult. eassumption. omega.
+      simpl in *. rewrite app_length. eapply closed_extend_mult. eassumption. omega. eauto.
 
   - Case "sub". subst.
     assert ((exists x : id, t0 = tvar true x) \/
                (exists (G' : venv) (t' : tm) n2,
-                  step G1 t0 (G'++G1) t' /\ has_type [] (G'++G1) t' T1 n2)) as HH.
+                  step G1 t0 (G'++G1) t' /\ has_type [] (G'++G1) t' T1 n2 /\ wf_sto (G'++G1))) as HH.
     eapply IHhas_type; eauto. change 0 with (length ([]:tenv)) at 1. eapply stpd2_closed1; eauto.
     destruct HH.
     + SCase "val".
       ev. subst. left. eexists. eauto.
     + SCase "step".
       ev. subst. 
-      right. repeat eexists. eauto. eapply T_Sub. eauto. eapply stp2_extend_mult. eauto. 
+      right. repeat eexists. eauto. eapply T_Sub. eauto. eapply stp2_extend_mult. eauto. eauto.
 Qed. 
 
 
